QCP_examples/humaneval/spec_logic_rewrite_c_files/C_89_goal.v
@@ -1,0 +1,627 @@
+Require Import Coq.ZArith.ZArith.
+Require Import Coq.Bool.Bool.
+Require Import Coq.Strings.String.
+Require Import Coq.Strings.Ascii.
+Require Import Coq.Lists.List.
+Require Import Coq.Classes.RelationClasses.
+Require Import Coq.Classes.Morphisms.
+Require Import Coq.micromega.Psatz.
+Require Import Coq.Sorting.Permutation.
+From AUXLib Require Import int_auto Axioms Feq Idents ListLib VMap.
+Require Import SetsClass.SetsClass. Import SetsNotation.
+From SimpleC.SL Require Import Mem SeparationLogic.
+Require Import Logic.LogicGenerator.demo932.Interface.
+Local Open Scope Z_scope.
+Local Open Scope sets.
+Local Open Scope string_scope.
+Local Open Scope list.
+Import naive_C_Rules.
+Require Import SimpleC.StdLib.string_lib.
+Require Import coins_89.
+Local Open Scope sac.
+From SimpleC.EE.QCP_demos_LLM Require Import char_array_strategy_goal.
+From SimpleC.EE.QCP_demos_LLM Require Import char_array_strategy_proof.
+From SimpleC.StdLib Require Import string_strategy_goal.
+From SimpleC.StdLib Require Import string_strategy_proof.
+
+(*----- Function encrypt -----*)
+
+Definition encrypt_safety_wit_1 := 
+forall (s_pre: Z) (input: (@list Z)) (retval: Z) (PreH1 : (retval = (string_length (input)))) (PreH2 : (0 <= ((string_length (input)) + 1 ))) (PreH3 : (valid_string input )) (PreH4 : (problem_89_pre_z input )) (PreH5 : (ascii_range_z input )) (PreH6 : ((string_length (input)) < INT_MAX)) ,
+  ((( &( "out" ) )) # Ptr  |->_)
+  **  (store_string s_pre input )
+  **  ((( &( "n" ) )) # Int  |-> retval)
+  **  ((( &( "s" ) )) # Ptr  |-> s_pre)
+|--
+  “ ((retval + 1 ) <= INT_MAX) ” 
+  &&  “ ((INT_MIN) <= (retval + 1 )) ”
+.
+
+Definition encrypt_safety_wit_2 := 
+forall (s_pre: Z) (input: (@list Z)) (retval: Z) (PreH1 : (retval = (string_length (input)))) (PreH2 : (0 <= ((string_length (input)) + 1 ))) (PreH3 : (valid_string input )) (PreH4 : (problem_89_pre_z input )) (PreH5 : (ascii_range_z input )) (PreH6 : ((string_length (input)) < INT_MAX)) ,
+  ((( &( "out" ) )) # Ptr  |->_)
+  **  (store_string s_pre input )
+  **  ((( &( "n" ) )) # Int  |-> retval)
+  **  ((( &( "s" ) )) # Ptr  |-> s_pre)
+|--
+  “ (1 <= INT_MAX) ” 
+  &&  “ ((INT_MIN) <= 1) ”
+.
+
+Definition encrypt_safety_wit_3 := 
+forall (s_pre: Z) (input: (@list Z)) (retval: Z) (retval_2: Z) (PreH1 : (retval_2 <> 0)) (PreH2 : (retval = (string_length (input)))) (PreH3 : (0 <= ((string_length (input)) + 1 ))) (PreH4 : (valid_string input )) (PreH5 : (problem_89_pre_z input )) (PreH6 : (ascii_range_z input )) (PreH7 : ((string_length (input)) < INT_MAX)) ,
+  (CharArray.undef_full retval_2 (retval + 1 ) )
+  **  (CharArray.full s_pre ((string_length (input)) + 1 ) (c_string (input)) )
+  **  ((( &( "out" ) )) # Ptr  |-> retval_2)
+  **  ((( &( "n" ) )) # Int  |-> retval)
+  **  ((( &( "s" ) )) # Ptr  |-> s_pre)
+|--
+  “ (0 <= INT_MAX) ” 
+  &&  “ ((INT_MIN) <= 0) ”
+.
+
+Definition encrypt_safety_wit_4 := 
+forall (s_pre: Z) (input: (@list Z)) (retval: Z) (retval_2: Z) (PreH1 : (retval_2 = 0)) (PreH2 : (retval_2 <> 0)) (PreH3 : (retval = (string_length (input)))) (PreH4 : (0 <= ((string_length (input)) + 1 ))) (PreH5 : (valid_string input )) (PreH6 : (problem_89_pre_z input )) (PreH7 : (ascii_range_z input )) (PreH8 : ((string_length (input)) < INT_MAX)) ,
+  (CharArray.undef_full retval_2 (retval + 1 ) )
+  **  (CharArray.full s_pre ((string_length (input)) + 1 ) (c_string (input)) )
+  **  ((( &( "out" ) )) # Ptr  |-> retval_2)
+  **  ((( &( "n" ) )) # Int  |-> retval)
+  **  ((( &( "s" ) )) # Ptr  |-> s_pre)
+|--
+  “ False ”
+.
+
+Definition encrypt_safety_wit_5 := 
+forall (s_pre: Z) (input: (@list Z)) (retval: Z) (retval_2: Z) (PreH1 : (retval_2 <> 0)) (PreH2 : (retval_2 <> 0)) (PreH3 : (retval = (string_length (input)))) (PreH4 : (0 <= ((string_length (input)) + 1 ))) (PreH5 : (valid_string input )) (PreH6 : (problem_89_pre_z input )) (PreH7 : (ascii_range_z input )) (PreH8 : ((string_length (input)) < INT_MAX)) ,
+  ((( &( "i" ) )) # Int  |->_)
+  **  (CharArray.undef_full retval_2 (retval + 1 ) )
+  **  (CharArray.full s_pre ((string_length (input)) + 1 ) (c_string (input)) )
+  **  ((( &( "out" ) )) # Ptr  |-> retval_2)
+  **  ((( &( "n" ) )) # Int  |-> retval)
+  **  ((( &( "s" ) )) # Ptr  |-> s_pre)
+|--
+  “ (0 <= INT_MAX) ” 
+  &&  “ ((INT_MIN) <= 0) ”
+.
+
+Definition encrypt_safety_wit_6 := 
+(
+forall (s_pre: Z) (input: (@list Z)) (out: Z) (output: (@list Z)) (i: Z) (n: Z) (PreH1 : (i < n)) (PreH2 : (n = (string_length (input)))) (PreH3 : (valid_string input )) (PreH4 : (problem_89_pre_z input )) (PreH5 : (ascii_range_z input )) (PreH6 : (lowercase_codes_z_89 input )) (PreH7 : ((string_length (input)) < INT_MAX)) (PreH8 : (0 <= i)) (PreH9 : (i <= n)) (PreH10 : (rotate_prefix_z_89 input output i )) ,
+  ((( &( "w" ) )) # Int  |->_)
+  **  ((( &( "s" ) )) # Ptr  |-> s_pre)
+  **  ((( &( "n" ) )) # Int  |-> n)
+  **  ((( &( "i" ) )) # Int  |-> i)
+  **  (store_string s_pre input )
+  **  ((( &( "out" ) )) # Ptr  |-> out)
+  **  (CharArray.full out i output )
+  **  (CharArray.undef_seg out i (n + 1 ) )
+|--
+  “ ((((((Znth i (c_string (input)) 0) + 4 ) - 97 ) % ( 26 ) ) + 97 ) <= INT_MAX) ” 
+  &&  “ ((INT_MIN) <= (((((Znth i (c_string (input)) 0) + 4 ) - 97 ) % ( 26 ) ) + 97 )) ”
+) \/
+(
+forall (s_pre: Z) (input: (@list Z)) (out: Z) (output: (@list Z)) (i: Z) (n: Z) (PreH1 : (i < n)) (PreH2 : (n = (string_length (input)))) (PreH3 : (valid_string input )) (PreH4 : (problem_89_pre_z input )) (PreH5 : (ascii_range_z input )) (PreH6 : (lowercase_codes_z_89 input )) (PreH7 : ((string_length (input)) < INT_MAX)) (PreH8 : (0 <= i)) (PreH9 : (i <= n)) (PreH10 : (rotate_prefix_z_89 input output i )) ,
+  ((( &( "w" ) )) # Int  |->_)
+  **  ((( &( "s" ) )) # Ptr  |-> s_pre)
+  **  ((( &( "n" ) )) # Int  |-> n)
+  **  ((( &( "i" ) )) # Int  |-> i)
+  **  (store_string s_pre input )
+  **  ((( &( "out" ) )) # Ptr  |-> out)
+  **  (CharArray.full out i output )
+  **  (CharArray.undef_seg out i (n + 1 ) )
+|--
+  “ ((((((Znth i (c_string (input)) 0) + 4 ) - 97 ) % ( 26 ) ) + 97 ) <= INT_MAX) ” 
+  &&  “ ((INT_MIN) <= (((((Znth i (c_string (input)) 0) + 4 ) - 97 ) % ( 26 ) ) + 97 )) ”
+).
+
+Definition encrypt_safety_wit_6_split_goal_1 := 
+forall (s_pre: Z) (input: (@list Z)) (out: Z) (output: (@list Z)) (i: Z) (n: Z) (PreH1 : (i < n)) (PreH2 : (n = (string_length (input)))) (PreH3 : (valid_string input )) (PreH4 : (problem_89_pre_z input )) (PreH5 : (ascii_range_z input )) (PreH6 : (lowercase_codes_z_89 input )) (PreH7 : ((string_length (input)) < INT_MAX)) (PreH8 : (0 <= i)) (PreH9 : (i <= n)) (PreH10 : (rotate_prefix_z_89 input output i )) ,
+  ((( &( "w" ) )) # Int  |->_)
+  **  ((( &( "s" ) )) # Ptr  |-> s_pre)
+  **  ((( &( "n" ) )) # Int  |-> n)
+  **  ((( &( "i" ) )) # Int  |-> i)
+  **  (store_string s_pre input )
+  **  ((( &( "out" ) )) # Ptr  |-> out)
+  **  (CharArray.full out i output )
+  **  (CharArray.undef_seg out i (n + 1 ) )
+|--
+  “ ((((((Znth i (c_string (input)) 0) + 4 ) - 97 ) % ( 26 ) ) + 97 ) <= INT_MAX) ”
+.
+
+Definition encrypt_safety_wit_6_split_goal_2 := 
+forall (s_pre: Z) (input: (@list Z)) (out: Z) (output: (@list Z)) (i: Z) (n: Z) (PreH1 : (i < n)) (PreH2 : (n = (string_length (input)))) (PreH3 : (valid_string input )) (PreH4 : (problem_89_pre_z input )) (PreH5 : (ascii_range_z input )) (PreH6 : (lowercase_codes_z_89 input )) (PreH7 : ((string_length (input)) < INT_MAX)) (PreH8 : (0 <= i)) (PreH9 : (i <= n)) (PreH10 : (rotate_prefix_z_89 input output i )) ,
+  ((( &( "w" ) )) # Int  |->_)
+  **  ((( &( "s" ) )) # Ptr  |-> s_pre)
+  **  ((( &( "n" ) )) # Int  |-> n)
+  **  ((( &( "i" ) )) # Int  |-> i)
+  **  (store_string s_pre input )
+  **  ((( &( "out" ) )) # Ptr  |-> out)
+  **  (CharArray.full out i output )
+  **  (CharArray.undef_seg out i (n + 1 ) )
+|--
+  “ ((INT_MIN) <= (((((Znth i (c_string (input)) 0) + 4 ) - 97 ) % ( 26 ) ) + 97 )) ”
+.
+
+Definition encrypt_safety_wit_7 := 
+forall (s_pre: Z) (input: (@list Z)) (out: Z) (output: (@list Z)) (i: Z) (n: Z) (PreH1 : (i < n)) (PreH2 : (n = (string_length (input)))) (PreH3 : (valid_string input )) (PreH4 : (problem_89_pre_z input )) (PreH5 : (ascii_range_z input )) (PreH6 : (lowercase_codes_z_89 input )) (PreH7 : ((string_length (input)) < INT_MAX)) (PreH8 : (0 <= i)) (PreH9 : (i <= n)) (PreH10 : (rotate_prefix_z_89 input output i )) ,
+  ((( &( "w" ) )) # Int  |->_)
+  **  ((( &( "s" ) )) # Ptr  |-> s_pre)
+  **  ((( &( "n" ) )) # Int  |-> n)
+  **  ((( &( "i" ) )) # Int  |-> i)
+  **  (store_string s_pre input )
+  **  ((( &( "out" ) )) # Ptr  |-> out)
+  **  (CharArray.full out i output )
+  **  (CharArray.undef_seg out i (n + 1 ) )
+|--
+  “ (((((Znth i (c_string (input)) 0) + 4 ) - 97 ) <> (INT_MIN)) \/ (26 <> (-1))) ” 
+  &&  “ (26 <> 0) ”
+.
+
+Definition encrypt_safety_wit_8 := 
+(
+forall (s_pre: Z) (input: (@list Z)) (out: Z) (output: (@list Z)) (i: Z) (n: Z) (PreH1 : (i < n)) (PreH2 : (n = (string_length (input)))) (PreH3 : (valid_string input )) (PreH4 : (problem_89_pre_z input )) (PreH5 : (ascii_range_z input )) (PreH6 : (lowercase_codes_z_89 input )) (PreH7 : ((string_length (input)) < INT_MAX)) (PreH8 : (0 <= i)) (PreH9 : (i <= n)) (PreH10 : (rotate_prefix_z_89 input output i )) ,
+  ((( &( "w" ) )) # Int  |->_)
+  **  ((( &( "s" ) )) # Ptr  |-> s_pre)
+  **  ((( &( "n" ) )) # Int  |-> n)
+  **  ((( &( "i" ) )) # Int  |-> i)
+  **  (store_string s_pre input )
+  **  ((( &( "out" ) )) # Ptr  |-> out)
+  **  (CharArray.full out i output )
+  **  (CharArray.undef_seg out i (n + 1 ) )
+|--
+  “ ((((Znth i (c_string (input)) 0) + 4 ) - 97 ) <= INT_MAX) ” 
+  &&  “ ((INT_MIN) <= (((Znth i (c_string (input)) 0) + 4 ) - 97 )) ”
+) \/
+(
+forall (s_pre: Z) (input: (@list Z)) (out: Z) (output: (@list Z)) (i: Z) (n: Z) (PreH1 : (i < n)) (PreH2 : (n = (string_length (input)))) (PreH3 : (valid_string input )) (PreH4 : (problem_89_pre_z input )) (PreH5 : (ascii_range_z input )) (PreH6 : (lowercase_codes_z_89 input )) (PreH7 : ((string_length (input)) < INT_MAX)) (PreH8 : (0 <= i)) (PreH9 : (i <= n)) (PreH10 : (rotate_prefix_z_89 input output i )) ,
+  ((( &( "w" ) )) # Int  |->_)
+  **  ((( &( "s" ) )) # Ptr  |-> s_pre)
+  **  ((( &( "n" ) )) # Int  |-> n)
+  **  ((( &( "i" ) )) # Int  |-> i)
+  **  (store_string s_pre input )
+  **  ((( &( "out" ) )) # Ptr  |-> out)
+  **  (CharArray.full out i output )
+  **  (CharArray.undef_seg out i (n + 1 ) )
+|--
+  “ ((((Znth i (c_string (input)) 0) + 4 ) - 97 ) <= INT_MAX) ” 
+  &&  “ ((INT_MIN) <= (((Znth i (c_string (input)) 0) + 4 ) - 97 )) ”
+).
+
+Definition encrypt_safety_wit_8_split_goal_1 := 
+forall (s_pre: Z) (input: (@list Z)) (out: Z) (output: (@list Z)) (i: Z) (n: Z) (PreH1 : (i < n)) (PreH2 : (n = (string_length (input)))) (PreH3 : (valid_string input )) (PreH4 : (problem_89_pre_z input )) (PreH5 : (ascii_range_z input )) (PreH6 : (lowercase_codes_z_89 input )) (PreH7 : ((string_length (input)) < INT_MAX)) (PreH8 : (0 <= i)) (PreH9 : (i <= n)) (PreH10 : (rotate_prefix_z_89 input output i )) ,
+  ((( &( "w" ) )) # Int  |->_)
+  **  ((( &( "s" ) )) # Ptr  |-> s_pre)
+  **  ((( &( "n" ) )) # Int  |-> n)
+  **  ((( &( "i" ) )) # Int  |-> i)
+  **  (store_string s_pre input )
+  **  ((( &( "out" ) )) # Ptr  |-> out)
+  **  (CharArray.full out i output )
+  **  (CharArray.undef_seg out i (n + 1 ) )
+|--
+  “ ((((Znth i (c_string (input)) 0) + 4 ) - 97 ) <= INT_MAX) ”
+.
+
+Definition encrypt_safety_wit_8_split_goal_2 := 
+forall (s_pre: Z) (input: (@list Z)) (out: Z) (output: (@list Z)) (i: Z) (n: Z) (PreH1 : (i < n)) (PreH2 : (n = (string_length (input)))) (PreH3 : (valid_string input )) (PreH4 : (problem_89_pre_z input )) (PreH5 : (ascii_range_z input )) (PreH6 : (lowercase_codes_z_89 input )) (PreH7 : ((string_length (input)) < INT_MAX)) (PreH8 : (0 <= i)) (PreH9 : (i <= n)) (PreH10 : (rotate_prefix_z_89 input output i )) ,
+  ((( &( "w" ) )) # Int  |->_)
+  **  ((( &( "s" ) )) # Ptr  |-> s_pre)
+  **  ((( &( "n" ) )) # Int  |-> n)
+  **  ((( &( "i" ) )) # Int  |-> i)
+  **  (store_string s_pre input )
+  **  ((( &( "out" ) )) # Ptr  |-> out)
+  **  (CharArray.full out i output )
+  **  (CharArray.undef_seg out i (n + 1 ) )
+|--
+  “ ((INT_MIN) <= (((Znth i (c_string (input)) 0) + 4 ) - 97 )) ”
+.
+
+Definition encrypt_safety_wit_9 := 
+(
+forall (s_pre: Z) (input: (@list Z)) (out: Z) (output: (@list Z)) (i: Z) (n: Z) (PreH1 : (i < n)) (PreH2 : (n = (string_length (input)))) (PreH3 : (valid_string input )) (PreH4 : (problem_89_pre_z input )) (PreH5 : (ascii_range_z input )) (PreH6 : (lowercase_codes_z_89 input )) (PreH7 : ((string_length (input)) < INT_MAX)) (PreH8 : (0 <= i)) (PreH9 : (i <= n)) (PreH10 : (rotate_prefix_z_89 input output i )) ,
+  ((( &( "w" ) )) # Int  |->_)
+  **  ((( &( "s" ) )) # Ptr  |-> s_pre)
+  **  ((( &( "n" ) )) # Int  |-> n)
+  **  ((( &( "i" ) )) # Int  |-> i)
+  **  (store_string s_pre input )
+  **  ((( &( "out" ) )) # Ptr  |-> out)
+  **  (CharArray.full out i output )
+  **  (CharArray.undef_seg out i (n + 1 ) )
+|--
+  “ (((Znth i (c_string (input)) 0) + 4 ) <= INT_MAX) ” 
+  &&  “ ((INT_MIN) <= ((Znth i (c_string (input)) 0) + 4 )) ”
+) \/
+(
+forall (s_pre: Z) (input: (@list Z)) (out: Z) (output: (@list Z)) (i: Z) (n: Z) (PreH1 : (i < n)) (PreH2 : (n = (string_length (input)))) (PreH3 : (valid_string input )) (PreH4 : (problem_89_pre_z input )) (PreH5 : (ascii_range_z input )) (PreH6 : (lowercase_codes_z_89 input )) (PreH7 : ((string_length (input)) < INT_MAX)) (PreH8 : (0 <= i)) (PreH9 : (i <= n)) (PreH10 : (rotate_prefix_z_89 input output i )) ,
+  ((( &( "w" ) )) # Int  |->_)
+  **  ((( &( "s" ) )) # Ptr  |-> s_pre)
+  **  ((( &( "n" ) )) # Int  |-> n)
+  **  ((( &( "i" ) )) # Int  |-> i)
+  **  (store_string s_pre input )
+  **  ((( &( "out" ) )) # Ptr  |-> out)
+  **  (CharArray.full out i output )
+  **  (CharArray.undef_seg out i (n + 1 ) )
+|--
+  “ (((Znth i (c_string (input)) 0) + 4 ) <= INT_MAX) ” 
+  &&  “ ((INT_MIN) <= ((Znth i (c_string (input)) 0) + 4 )) ”
+).
+
+Definition encrypt_safety_wit_9_split_goal_1 := 
+forall (s_pre: Z) (input: (@list Z)) (out: Z) (output: (@list Z)) (i: Z) (n: Z) (PreH1 : (i < n)) (PreH2 : (n = (string_length (input)))) (PreH3 : (valid_string input )) (PreH4 : (problem_89_pre_z input )) (PreH5 : (ascii_range_z input )) (PreH6 : (lowercase_codes_z_89 input )) (PreH7 : ((string_length (input)) < INT_MAX)) (PreH8 : (0 <= i)) (PreH9 : (i <= n)) (PreH10 : (rotate_prefix_z_89 input output i )) ,
+  ((( &( "w" ) )) # Int  |->_)
+  **  ((( &( "s" ) )) # Ptr  |-> s_pre)
+  **  ((( &( "n" ) )) # Int  |-> n)
+  **  ((( &( "i" ) )) # Int  |-> i)
+  **  (store_string s_pre input )
+  **  ((( &( "out" ) )) # Ptr  |-> out)
+  **  (CharArray.full out i output )
+  **  (CharArray.undef_seg out i (n + 1 ) )
+|--
+  “ (((Znth i (c_string (input)) 0) + 4 ) <= INT_MAX) ”
+.
+
+Definition encrypt_safety_wit_9_split_goal_2 := 
+forall (s_pre: Z) (input: (@list Z)) (out: Z) (output: (@list Z)) (i: Z) (n: Z) (PreH1 : (i < n)) (PreH2 : (n = (string_length (input)))) (PreH3 : (valid_string input )) (PreH4 : (problem_89_pre_z input )) (PreH5 : (ascii_range_z input )) (PreH6 : (lowercase_codes_z_89 input )) (PreH7 : ((string_length (input)) < INT_MAX)) (PreH8 : (0 <= i)) (PreH9 : (i <= n)) (PreH10 : (rotate_prefix_z_89 input output i )) ,
+  ((( &( "w" ) )) # Int  |->_)
+  **  ((( &( "s" ) )) # Ptr  |-> s_pre)
+  **  ((( &( "n" ) )) # Int  |-> n)
+  **  ((( &( "i" ) )) # Int  |-> i)
+  **  (store_string s_pre input )
+  **  ((( &( "out" ) )) # Ptr  |-> out)
+  **  (CharArray.full out i output )
+  **  (CharArray.undef_seg out i (n + 1 ) )
+|--
+  “ ((INT_MIN) <= ((Znth i (c_string (input)) 0) + 4 )) ”
+.
+
+Definition encrypt_safety_wit_10 := 
+forall (s_pre: Z) (input: (@list Z)) (out: Z) (output: (@list Z)) (i: Z) (n: Z) (PreH1 : (i < n)) (PreH2 : (n = (string_length (input)))) (PreH3 : (valid_string input )) (PreH4 : (problem_89_pre_z input )) (PreH5 : (ascii_range_z input )) (PreH6 : (lowercase_codes_z_89 input )) (PreH7 : ((string_length (input)) < INT_MAX)) (PreH8 : (0 <= i)) (PreH9 : (i <= n)) (PreH10 : (rotate_prefix_z_89 input output i )) ,
+  ((( &( "w" ) )) # Int  |->_)
+  **  ((( &( "s" ) )) # Ptr  |-> s_pre)
+  **  ((( &( "n" ) )) # Int  |-> n)
+  **  ((( &( "i" ) )) # Int  |-> i)
+  **  (store_string s_pre input )
+  **  ((( &( "out" ) )) # Ptr  |-> out)
+  **  (CharArray.full out i output )
+  **  (CharArray.undef_seg out i (n + 1 ) )
+|--
+  “ (4 <= INT_MAX) ” 
+  &&  “ ((INT_MIN) <= 4) ”
+.
+
+Definition encrypt_safety_wit_11 := 
+forall (s_pre: Z) (input: (@list Z)) (out: Z) (output: (@list Z)) (i: Z) (n: Z) (PreH1 : (i < n)) (PreH2 : (n = (string_length (input)))) (PreH3 : (valid_string input )) (PreH4 : (problem_89_pre_z input )) (PreH5 : (ascii_range_z input )) (PreH6 : (lowercase_codes_z_89 input )) (PreH7 : ((string_length (input)) < INT_MAX)) (PreH8 : (0 <= i)) (PreH9 : (i <= n)) (PreH10 : (rotate_prefix_z_89 input output i )) ,
+  ((( &( "w" ) )) # Int  |->_)
+  **  ((( &( "s" ) )) # Ptr  |-> s_pre)
+  **  ((( &( "n" ) )) # Int  |-> n)
+  **  ((( &( "i" ) )) # Int  |-> i)
+  **  (store_string s_pre input )
+  **  ((( &( "out" ) )) # Ptr  |-> out)
+  **  (CharArray.full out i output )
+  **  (CharArray.undef_seg out i (n + 1 ) )
+|--
+  “ (97 <= INT_MAX) ” 
+  &&  “ ((INT_MIN) <= 97) ”
+.
+
+Definition encrypt_safety_wit_12 := 
+forall (s_pre: Z) (input: (@list Z)) (out: Z) (output: (@list Z)) (i: Z) (n: Z) (PreH1 : (i < n)) (PreH2 : (n = (string_length (input)))) (PreH3 : (valid_string input )) (PreH4 : (problem_89_pre_z input )) (PreH5 : (ascii_range_z input )) (PreH6 : (lowercase_codes_z_89 input )) (PreH7 : ((string_length (input)) < INT_MAX)) (PreH8 : (0 <= i)) (PreH9 : (i <= n)) (PreH10 : (rotate_prefix_z_89 input output i )) ,
+  ((( &( "w" ) )) # Int  |->_)
+  **  ((( &( "s" ) )) # Ptr  |-> s_pre)
+  **  ((( &( "n" ) )) # Int  |-> n)
+  **  ((( &( "i" ) )) # Int  |-> i)
+  **  (store_string s_pre input )
+  **  ((( &( "out" ) )) # Ptr  |-> out)
+  **  (CharArray.full out i output )
+  **  (CharArray.undef_seg out i (n + 1 ) )
+|--
+  “ (26 <= INT_MAX) ” 
+  &&  “ ((INT_MIN) <= 26) ”
+.
+
+Definition encrypt_safety_wit_13 := 
+forall (s_pre: Z) (input: (@list Z)) (out: Z) (output: (@list Z)) (i: Z) (n: Z) (PreH1 : (i < n)) (PreH2 : (n = (string_length (input)))) (PreH3 : (valid_string input )) (PreH4 : (problem_89_pre_z input )) (PreH5 : (ascii_range_z input )) (PreH6 : (lowercase_codes_z_89 input )) (PreH7 : ((string_length (input)) < INT_MAX)) (PreH8 : (0 <= i)) (PreH9 : (i <= n)) (PreH10 : (rotate_prefix_z_89 input output i )) ,
+  ((( &( "w" ) )) # Int  |->_)
+  **  ((( &( "s" ) )) # Ptr  |-> s_pre)
+  **  ((( &( "n" ) )) # Int  |-> n)
+  **  ((( &( "i" ) )) # Int  |-> i)
+  **  (store_string s_pre input )
+  **  ((( &( "out" ) )) # Ptr  |-> out)
+  **  (CharArray.full out i output )
+  **  (CharArray.undef_seg out i (n + 1 ) )
+|--
+  “ (97 <= INT_MAX) ” 
+  &&  “ ((INT_MIN) <= 97) ”
+.
+
+Definition encrypt_safety_wit_14 := 
+forall (s_pre: Z) (input: (@list Z)) (out: Z) (output: (@list Z)) (i: Z) (n: Z) (PreH1 : (0 <= ((string_length (input)) + 1 ))) (PreH2 : (i < n)) (PreH3 : (n = (string_length (input)))) (PreH4 : (valid_string input )) (PreH5 : (problem_89_pre_z input )) (PreH6 : (ascii_range_z input )) (PreH7 : (lowercase_codes_z_89 input )) (PreH8 : ((string_length (input)) < INT_MAX)) (PreH9 : (0 <= i)) (PreH10 : (i <= n)) (PreH11 : (rotate_prefix_z_89 input output i )) ,
+  (CharArray.full out (i + 1 ) (app (output) ((cons ((signed_last_nbits ((((((Znth i (c_string (input)) 0) + 4 ) - 97 ) % ( 26 ) ) + 97 )) (8))) ((@nil Z))))) )
+  **  (CharArray.undef_seg out (i + 1 ) (n + 1 ) )
+  **  (CharArray.full s_pre ((string_length (input)) + 1 ) (c_string (input)) )
+  **  ((( &( "s" ) )) # Ptr  |-> s_pre)
+  **  ((( &( "n" ) )) # Int  |-> n)
+  **  ((( &( "i" ) )) # Int  |-> i)
+  **  ((( &( "out" ) )) # Ptr  |-> out)
+|--
+  “ ((i + 1 ) <= INT_MAX) ” 
+  &&  “ ((INT_MIN) <= (i + 1 )) ”
+.
+
+Definition encrypt_safety_wit_15 := 
+forall (s_pre: Z) (input: (@list Z)) (out: Z) (output: (@list Z)) (i: Z) (n: Z) (PreH1 : (i >= n)) (PreH2 : (n = (string_length (input)))) (PreH3 : (valid_string input )) (PreH4 : (problem_89_pre_z input )) (PreH5 : (ascii_range_z input )) (PreH6 : (lowercase_codes_z_89 input )) (PreH7 : ((string_length (input)) < INT_MAX)) (PreH8 : (0 <= i)) (PreH9 : (i <= n)) (PreH10 : (rotate_prefix_z_89 input output i )) ,
+  ((( &( "s" ) )) # Ptr  |-> s_pre)
+  **  ((( &( "n" ) )) # Int  |-> n)
+  **  ((( &( "i" ) )) # Int  |-> i)
+  **  (store_string s_pre input )
+  **  ((( &( "out" ) )) # Ptr  |-> out)
+  **  (CharArray.full out i output )
+  **  (CharArray.undef_seg out i (n + 1 ) )
+|--
+  “ (0 <= INT_MAX) ” 
+  &&  “ ((INT_MIN) <= 0) ”
+.
+
+Definition encrypt_entail_wit_1 := 
+(
+forall (s_pre: Z) (input: (@list Z)) (retval: Z) (retval_2: Z) (PreH1 : (retval_2 <> 0)) (PreH2 : (retval_2 <> 0)) (PreH3 : (retval = (string_length (input)))) (PreH4 : (0 <= ((string_length (input)) + 1 ))) (PreH5 : (valid_string input )) (PreH6 : (problem_89_pre_z input )) (PreH7 : (ascii_range_z input )) (PreH8 : ((string_length (input)) < INT_MAX)) ,
+  (CharArray.undef_full retval_2 (retval + 1 ) )
+  **  (CharArray.full s_pre ((string_length (input)) + 1 ) (c_string (input)) )
+|--
+  EX (output: (@list Z)) ,
+  “ (retval = (string_length (input))) ” 
+  &&  “ (valid_string input ) ” 
+  &&  “ (problem_89_pre_z input ) ” 
+  &&  “ (ascii_range_z input ) ” 
+  &&  “ (lowercase_codes_z_89 input ) ” 
+  &&  “ ((string_length (input)) < INT_MAX) ” 
+  &&  “ (0 <= 0) ” 
+  &&  “ (0 <= retval) ” 
+  &&  “ (rotate_prefix_z_89 input output 0 ) ”
+  &&  (store_string s_pre input )
+  **  (CharArray.full retval_2 0 output )
+  **  (CharArray.undef_seg retval_2 0 (retval + 1 ) )
+) \/
+(
+forall (input: (@list Z)) (retval: Z) (retval_2: Z) (PreH1 : (retval_2 <> 0)) (PreH2 : (retval_2 <> 0)) (PreH3 : (retval = (string_length (input)))) (PreH4 : (0 <= ((string_length (input)) + 1 ))) (PreH5 : (valid_string input )) (PreH6 : (problem_89_pre_z input )) (PreH7 : (ascii_range_z input )) (PreH8 : ((string_length (input)) < INT_MAX)) ,
+  (CharArray.undef_full retval_2 (retval + 1 ) )
+|--
+  “ (rotate_prefix_z_89 input (@nil Z) 0 ) ” 
+  &&  “ (0 <= retval) ” 
+  &&  “ (lowercase_codes_z_89 input ) ”
+  &&  (CharArray.undef_full retval_2 (retval + 1 ) )
+).
+
+Definition encrypt_entail_wit_1_split_goal_1 := 
+forall (input: (@list Z)) (retval: Z) (retval_2: Z) (PreH1 : (retval_2 <> 0)) (PreH2 : (retval_2 <> 0)) (PreH3 : (retval = (string_length (input)))) (PreH4 : (0 <= ((string_length (input)) + 1 ))) (PreH5 : (valid_string input )) (PreH6 : (problem_89_pre_z input )) (PreH7 : (ascii_range_z input )) (PreH8 : ((string_length (input)) < INT_MAX)) ,
+  (CharArray.undef_full retval_2 (retval + 1 ) )
+|--
+  “ (rotate_prefix_z_89 input (@nil Z) 0 ) ”
+.
+
+Definition encrypt_entail_wit_1_split_goal_2 := 
+forall (input: (@list Z)) (retval: Z) (retval_2: Z) (PreH1 : (retval_2 <> 0)) (PreH2 : (retval_2 <> 0)) (PreH3 : (retval = (string_length (input)))) (PreH4 : (0 <= ((string_length (input)) + 1 ))) (PreH5 : (valid_string input )) (PreH6 : (problem_89_pre_z input )) (PreH7 : (ascii_range_z input )) (PreH8 : ((string_length (input)) < INT_MAX)) ,
+  (CharArray.undef_full retval_2 (retval + 1 ) )
+|--
+  “ (0 <= retval) ”
+.
+
+Definition encrypt_entail_wit_1_split_goal_3 := 
+forall (input: (@list Z)) (retval: Z) (retval_2: Z) (PreH1 : (retval_2 <> 0)) (PreH2 : (retval_2 <> 0)) (PreH3 : (retval = (string_length (input)))) (PreH4 : (0 <= ((string_length (input)) + 1 ))) (PreH5 : (valid_string input )) (PreH6 : (problem_89_pre_z input )) (PreH7 : (ascii_range_z input )) (PreH8 : ((string_length (input)) < INT_MAX)) ,
+  (CharArray.undef_full retval_2 (retval + 1 ) )
+|--
+  “ (lowercase_codes_z_89 input ) ”
+.
+
+Definition encrypt_entail_wit_1_split_goal_spatial := 
+forall (input: (@list Z)) (retval: Z) (retval_2: Z) (PreH1 : (retval_2 <> 0)) (PreH2 : (retval_2 <> 0)) (PreH3 : (retval = (string_length (input)))) (PreH4 : (0 <= ((string_length (input)) + 1 ))) (PreH5 : (valid_string input )) (PreH6 : (problem_89_pre_z input )) (PreH7 : (ascii_range_z input )) (PreH8 : ((string_length (input)) < INT_MAX)) ,
+  (CharArray.undef_full retval_2 (retval + 1 ) )
+|--
+  (CharArray.undef_full retval_2 (retval + 1 ) )
+.
+
+Definition encrypt_entail_wit_2 := 
+(
+forall (s_pre: Z) (input: (@list Z)) (out: Z) (output_2: (@list Z)) (i: Z) (n: Z) (PreH1 : (0 <= ((string_length (input)) + 1 ))) (PreH2 : (i < n)) (PreH3 : (n = (string_length (input)))) (PreH4 : (valid_string input )) (PreH5 : (problem_89_pre_z input )) (PreH6 : (ascii_range_z input )) (PreH7 : (lowercase_codes_z_89 input )) (PreH8 : ((string_length (input)) < INT_MAX)) (PreH9 : (0 <= i)) (PreH10 : (i <= n)) (PreH11 : (rotate_prefix_z_89 input output_2 i )) ,
+  (CharArray.full out (i + 1 ) (app (output_2) ((cons ((signed_last_nbits ((((((Znth i (c_string (input)) 0) + 4 ) - 97 ) % ( 26 ) ) + 97 )) (8))) ((@nil Z))))) )
+  **  (CharArray.undef_seg out (i + 1 ) (n + 1 ) )
+  **  (CharArray.full s_pre ((string_length (input)) + 1 ) (c_string (input)) )
+|--
+  EX (output: (@list Z)) ,
+  “ (n = (string_length (input))) ” 
+  &&  “ (valid_string input ) ” 
+  &&  “ (problem_89_pre_z input ) ” 
+  &&  “ (ascii_range_z input ) ” 
+  &&  “ (lowercase_codes_z_89 input ) ” 
+  &&  “ ((string_length (input)) < INT_MAX) ” 
+  &&  “ (0 <= (i + 1 )) ” 
+  &&  “ ((i + 1 ) <= n) ” 
+  &&  “ (rotate_prefix_z_89 input output (i + 1 ) ) ”
+  &&  (store_string s_pre input )
+  **  (CharArray.full out (i + 1 ) output )
+  **  (CharArray.undef_seg out (i + 1 ) (n + 1 ) )
+) \/
+(
+forall (input: (@list Z)) (output_2: (@list Z)) (i: Z) (n: Z) (PreH1 : (0 <= ((string_length (input)) + 1 ))) (PreH2 : (i < n)) (PreH3 : (n = (string_length (input)))) (PreH4 : (valid_string input )) (PreH5 : (problem_89_pre_z input )) (PreH6 : (ascii_range_z input )) (PreH7 : (lowercase_codes_z_89 input )) (PreH8 : ((string_length (input)) < INT_MAX)) (PreH9 : (0 <= i)) (PreH10 : (i <= n)) (PreH11 : (rotate_prefix_z_89 input output_2 i )) ,
+  TT && emp 
+|--
+  “ (rotate_prefix_z_89 input (app (output_2) ((cons ((signed_last_nbits ((((((Znth i (c_string (input)) 0) + 4 ) - 97 ) % ( 26 ) ) + 97 )) (8))) ((@nil Z))))) (i + 1 ) ) ”
+  &&  emp
+).
+
+Definition encrypt_entail_wit_2_split_goal_1 := 
+forall (input: (@list Z)) (output_2: (@list Z)) (i: Z) (n: Z) (PreH1 : (0 <= ((string_length (input)) + 1 ))) (PreH2 : (i < n)) (PreH3 : (n = (string_length (input)))) (PreH4 : (valid_string input )) (PreH5 : (problem_89_pre_z input )) (PreH6 : (ascii_range_z input )) (PreH7 : (lowercase_codes_z_89 input )) (PreH8 : ((string_length (input)) < INT_MAX)) (PreH9 : (0 <= i)) (PreH10 : (i <= n)) (PreH11 : (rotate_prefix_z_89 input output_2 i )) ,
+  TT && emp 
+|--
+  “ (rotate_prefix_z_89 input (app (output_2) ((cons ((signed_last_nbits ((((((Znth i (c_string (input)) 0) + 4 ) - 97 ) % ( 26 ) ) + 97 )) (8))) ((@nil Z))))) (i + 1 ) ) ”
+.
+
+Definition encrypt_return_wit_1 := 
+(
+forall (s_pre: Z) (input: (@list Z)) (out: Z) (output_2: (@list Z)) (i: Z) (n: Z) (PreH1 : (0 <= ((string_length (input)) + 1 ))) (PreH2 : (i >= n)) (PreH3 : (n = (string_length (input)))) (PreH4 : (valid_string input )) (PreH5 : (problem_89_pre_z input )) (PreH6 : (ascii_range_z input )) (PreH7 : (lowercase_codes_z_89 input )) (PreH8 : ((string_length (input)) < INT_MAX)) (PreH9 : (0 <= i)) (PreH10 : (i <= n)) (PreH11 : (rotate_prefix_z_89 input output_2 i )) ,
+  (CharArray.full out (i + 1 ) (app (output_2) ((cons (0) ((@nil Z))))) )
+  **  (CharArray.undef_seg out (n + 1 ) (n + 1 ) )
+  **  (CharArray.full s_pre ((string_length (input)) + 1 ) (c_string (input)) )
+|--
+  EX (output: (@list Z)) ,
+  “ (problem_89_spec_z input output ) ”
+  &&  (store_string s_pre input )
+  **  (store_string out output )
+) \/
+(
+forall (input: (@list Z)) (out: Z) (output_2: (@list Z)) (i: Z) (n: Z) (PreH1 : (0 <= (i + 1 ))) (PreH2 : (0 <= ((string_length (input)) + 1 ))) (PreH3 : (i >= n)) (PreH4 : (n = (string_length (input)))) (PreH5 : (valid_string input )) (PreH6 : (problem_89_pre_z input )) (PreH7 : (ascii_range_z input )) (PreH8 : (lowercase_codes_z_89 input )) (PreH9 : ((string_length (input)) < INT_MAX)) (PreH10 : (0 <= i)) (PreH11 : (i <= n)) (PreH12 : (rotate_prefix_z_89 input output_2 i )) ,
+  (CharArray.full out (i + 1 ) (app (output_2) ((cons (0) ((@nil Z))))) )
+|--
+  EX (output: (@list Z)) ,
+  “ (problem_89_spec_z input output ) ”
+  &&  (CharArray.full out ((string_length (output)) + 1 ) (c_string (output)) )
+).
+
+Definition encrypt_partial_solve_wit_1_pure := 
+forall (s_pre: Z) (input: (@list Z)) (PreH1 : (valid_string input )) (PreH2 : (problem_89_pre_z input )) (PreH3 : (ascii_range_z input )) (PreH4 : ((string_length (input)) < INT_MAX)) ,
+  ((( &( "n" ) )) # Int  |->_)
+  **  ((( &( "s" ) )) # Ptr  |-> s_pre)
+  **  (store_string s_pre input )
+|--
+  “ (valid_string input ) ” 
+  &&  “ ((string_length (input)) < INT_MAX) ”
+.
+
+Definition encrypt_partial_solve_wit_1_aux := 
+forall (s_pre: Z) (input: (@list Z)) (PreH1 : (valid_string input )) (PreH2 : (problem_89_pre_z input )) (PreH3 : (ascii_range_z input )) (PreH4 : ((string_length (input)) < INT_MAX)) ,
+  (store_string s_pre input )
+|--
+  “ (valid_string input ) ” 
+  &&  “ ((string_length (input)) < INT_MAX) ” 
+  &&  “ (0 <= ((string_length (input)) + 1 )) ” 
+  &&  “ (valid_string input ) ” 
+  &&  “ (problem_89_pre_z input ) ” 
+  &&  “ (ascii_range_z input ) ” 
+  &&  “ ((string_length (input)) < INT_MAX) ”
+  &&  (store_string s_pre input )
+.
+
+Definition encrypt_partial_solve_wit_1 := encrypt_partial_solve_wit_1_pure -> encrypt_partial_solve_wit_1_aux.
+
+Definition encrypt_partial_solve_wit_2_pure := 
+(
+forall (s_pre: Z) (input: (@list Z)) (retval: Z) (PreH1 : (retval = (string_length (input)))) (PreH2 : (0 <= ((string_length (input)) + 1 ))) (PreH3 : (valid_string input )) (PreH4 : (problem_89_pre_z input )) (PreH5 : (ascii_range_z input )) (PreH6 : ((string_length (input)) < INT_MAX)) ,
+  ((( &( "out" ) )) # Ptr  |->_)
+  **  (store_string s_pre input )
+  **  ((( &( "n" ) )) # Int  |-> retval)
+  **  ((( &( "s" ) )) # Ptr  |-> s_pre)
+|--
+  “ ((retval + 1 ) > 0) ”
+) \/
+(
+forall (s_pre: Z) (input: (@list Z)) (retval: Z) (PreH1 : (retval <= INT_MAX)) (PreH2 : (retval >= INT_MIN)) (PreH3 : (retval = (string_length (input)))) (PreH4 : (0 <= ((string_length (input)) + 1 ))) (PreH5 : (valid_string input )) (PreH6 : (problem_89_pre_z input )) (PreH7 : (ascii_range_z input )) (PreH8 : ((string_length (input)) < INT_MAX)) ,
+  (CharArray.full s_pre ((string_length (input)) + 1 ) (c_string (input)) )
+  **  ((( &( "out" ) )) # Ptr  |->_)
+  **  ((( &( "n" ) )) # Int  |-> retval)
+  **  ((( &( "s" ) )) # Ptr  |-> s_pre)
+|--
+  “ ((retval + 1 ) > 0) ”
+).
+
+Definition encrypt_partial_solve_wit_2_pure_split_goal_1 := 
+forall (s_pre: Z) (input: (@list Z)) (retval: Z) (PreH1 : (retval <= INT_MAX)) (PreH2 : (retval >= INT_MIN)) (PreH3 : (retval = (string_length (input)))) (PreH4 : (0 <= ((string_length (input)) + 1 ))) (PreH5 : (valid_string input )) (PreH6 : (problem_89_pre_z input )) (PreH7 : (ascii_range_z input )) (PreH8 : ((string_length (input)) < INT_MAX)) ,
+  (CharArray.full s_pre ((string_length (input)) + 1 ) (c_string (input)) )
+  **  ((( &( "out" ) )) # Ptr  |->_)
+  **  ((( &( "n" ) )) # Int  |-> retval)
+  **  ((( &( "s" ) )) # Ptr  |-> s_pre)
+|--
+  “ ((retval + 1 ) > 0) ”
+.
+
+Definition encrypt_partial_solve_wit_2_aux := 
+forall (s_pre: Z) (input: (@list Z)) (retval: Z) (PreH1 : (retval = (string_length (input)))) (PreH2 : (0 <= ((string_length (input)) + 1 ))) (PreH3 : (valid_string input )) (PreH4 : (problem_89_pre_z input )) (PreH5 : (ascii_range_z input )) (PreH6 : ((string_length (input)) < INT_MAX)) ,
+  (store_string s_pre input )
+|--
+  “ ((retval + 1 ) > 0) ” 
+  &&  “ (retval = (string_length (input))) ” 
+  &&  “ (0 <= ((string_length (input)) + 1 )) ” 
+  &&  “ (valid_string input ) ” 
+  &&  “ (problem_89_pre_z input ) ” 
+  &&  “ (ascii_range_z input ) ” 
+  &&  “ ((string_length (input)) < INT_MAX) ”
+  &&  (CharArray.full s_pre ((string_length (input)) + 1 ) (c_string (input)) )
+.
+
+Definition encrypt_partial_solve_wit_2 := encrypt_partial_solve_wit_2_pure -> encrypt_partial_solve_wit_2_aux.
+
+Definition encrypt_partial_solve_wit_3 := 
+forall (s_pre: Z) (input: (@list Z)) (out: Z) (output: (@list Z)) (i: Z) (n: Z) (PreH1 : (i < n)) (PreH2 : (n = (string_length (input)))) (PreH3 : (valid_string input )) (PreH4 : (problem_89_pre_z input )) (PreH5 : (ascii_range_z input )) (PreH6 : (lowercase_codes_z_89 input )) (PreH7 : ((string_length (input)) < INT_MAX)) (PreH8 : (0 <= i)) (PreH9 : (i <= n)) (PreH10 : (rotate_prefix_z_89 input output i )) ,
+  (store_string s_pre input )
+  **  (CharArray.full out i output )
+  **  (CharArray.undef_seg out i (n + 1 ) )
+|--
+  “ (0 <= ((string_length (input)) + 1 )) ” 
+  &&  “ (i < n) ” 
+  &&  “ (n = (string_length (input))) ” 
+  &&  “ (valid_string input ) ” 
+  &&  “ (problem_89_pre_z input ) ” 
+  &&  “ (ascii_range_z input ) ” 
+  &&  “ (lowercase_codes_z_89 input ) ” 
+  &&  “ ((string_length (input)) < INT_MAX) ” 
+  &&  “ (0 <= i) ” 
+  &&  “ (i <= n) ” 
+  &&  “ (rotate_prefix_z_89 input output i ) ”
+  &&  (((out + (i * sizeof(CHAR) ) )) # Char  |->_)
+  **  (CharArray.full s_pre ((string_length (input)) + 1 ) (c_string (input)) )
+  **  (CharArray.undef_missing_i out i i (n + 1 ) )
+  **  (CharArray.full out i output )
+.
+
+Definition encrypt_partial_solve_wit_4 := 
+forall (s_pre: Z) (input: (@list Z)) (out: Z) (output: (@list Z)) (i: Z) (n: Z) (PreH1 : (i >= n)) (PreH2 : (n = (string_length (input)))) (PreH3 : (valid_string input )) (PreH4 : (problem_89_pre_z input )) (PreH5 : (ascii_range_z input )) (PreH6 : (lowercase_codes_z_89 input )) (PreH7 : ((string_length (input)) < INT_MAX)) (PreH8 : (0 <= i)) (PreH9 : (i <= n)) (PreH10 : (rotate_prefix_z_89 input output i )) ,
+  (store_string s_pre input )
+  **  (CharArray.full out i output )
+  **  (CharArray.undef_seg out i (n + 1 ) )
+|--
+  “ (0 <= ((string_length (input)) + 1 )) ” 
+  &&  “ (i >= n) ” 
+  &&  “ (n = (string_length (input))) ” 
+  &&  “ (valid_string input ) ” 
+  &&  “ (problem_89_pre_z input ) ” 
+  &&  “ (ascii_range_z input ) ” 
+  &&  “ (lowercase_codes_z_89 input ) ” 
+  &&  “ ((string_length (input)) < INT_MAX) ” 
+  &&  “ (0 <= i) ” 
+  &&  “ (i <= n) ” 
+  &&  “ (rotate_prefix_z_89 input output i ) ”
+  &&  (((out + (n * sizeof(CHAR) ) )) # Char  |->_)
+  **  (CharArray.full s_pre ((string_length (input)) + 1 ) (c_string (input)) )
+  **  (CharArray.undef_missing_i out n i (n + 1 ) )
+  **  (CharArray.full out i output )
+.
+
+Module Type VC_Correct.
+
+Include char_array_Strategy_Correct.
+Include string_Strategy_Correct.
+
+Axiom proof_of_encrypt_safety_wit_1 : encrypt_safety_wit_1.
+Axiom proof_of_encrypt_safety_wit_2 : encrypt_safety_wit_2.
+Axiom proof_of_encrypt_safety_wit_3 : encrypt_safety_wit_3.
+Axiom proof_of_encrypt_safety_wit_4 : encrypt_safety_wit_4.
+Axiom proof_of_encrypt_safety_wit_5 : encrypt_safety_wit_5.
+Axiom proof_of_encrypt_safety_wit_6 : encrypt_safety_wit_6.
+Axiom proof_of_encrypt_safety_wit_7 : encrypt_safety_wit_7.
+Axiom proof_of_encrypt_safety_wit_8 : encrypt_safety_wit_8.
+Axiom proof_of_encrypt_safety_wit_9 : encrypt_safety_wit_9.
+Axiom proof_of_encrypt_safety_wit_10 : encrypt_safety_wit_10.
+Axiom proof_of_encrypt_safety_wit_11 : encrypt_safety_wit_11.
+Axiom proof_of_encrypt_safety_wit_12 : encrypt_safety_wit_12.
+Axiom proof_of_encrypt_safety_wit_13 : encrypt_safety_wit_13.
+Axiom proof_of_encrypt_safety_wit_14 : encrypt_safety_wit_14.
+Axiom proof_of_encrypt_safety_wit_15 : encrypt_safety_wit_15.
+Axiom proof_of_encrypt_entail_wit_1 : encrypt_entail_wit_1.
+Axiom proof_of_encrypt_entail_wit_2 : encrypt_entail_wit_2.
+Axiom proof_of_encrypt_return_wit_1 : encrypt_return_wit_1.
+Axiom proof_of_encrypt_partial_solve_wit_1_pure : encrypt_partial_solve_wit_1_pure.
+Axiom proof_of_encrypt_partial_solve_wit_1 : encrypt_partial_solve_wit_1.
+Axiom proof_of_encrypt_partial_solve_wit_2_pure : encrypt_partial_solve_wit_2_pure.
+Axiom proof_of_encrypt_partial_solve_wit_2 : encrypt_partial_solve_wit_2.
+Axiom proof_of_encrypt_partial_solve_wit_3 : encrypt_partial_solve_wit_3.
+Axiom proof_of_encrypt_partial_solve_wit_4 : encrypt_partial_solve_wit_4.
+
+End VC_Correct.
